Refine the blame invariants and progress a bit in the proof of parallel_concrete

security/Blame.v
@@ -1,6 +1,6 @@
 Require Import String.
 Require Import Coqlib Maps Errors Integers.
-Require Import AST Linking Smallstep Events Behaviors Memory Values.
+Require Import AST Globalenvs Linking Smallstep Events Behaviors Memory Values.
 
 Require Import Ctypes Cop Clight.
 Require Import Split.
@@ -9,13 +9,23 @@ Definition same_domain (s: split) (j: meminj) (m: mem): Prop :=
   forall b cp, Mem.block_compartment m b = Some cp ->
           (j b <> None <-> s cp = Right).
 
+Definition delta_zero (j: meminj): Prop :=
+  forall loc loc' delta, j loc = Some (loc', delta) -> delta = 0.
+
+Definition same_symbols (j: meminj) (ge1 ge2: genv): Prop :=
+  forall id loc,
+    Genv.find_symbol ge1 id = Some loc ->
+    exists loc', j loc = Some (loc', 0) /\ Genv.find_symbol ge2 id = Some loc'.
+
 Section Equivalence.
   Variable s: split.
   Variable j: meminj.
 
-  Record right_mem_injection (m1 m2: mem) :=
+  Record right_mem_injection (ge1 ge2: genv) (m1 m2: mem) :=
     { same_dom: same_domain s j m1;
       partial_mem_inject: Mem.inject j m1 m2;
+      j_delta_zero: delta_zero j;
+      same_symb: same_symbols j ge1 ge2
     }.
 
 
@@ -51,11 +61,19 @@ Inductive right_cont_injection: cont -> cont -> Prop :=
     right_cont_injection (Kcall id1 f1 en1 le1 k1) (Kcall id2 f2 en2 le2 k2)
 .
 
-Definition right_env_injection (e1 e2: env): Prop :=
+Definition right_env_injection_some (e1 e2: env): Prop :=
   forall i b ty,
     e1 ! i = Some (b, ty) ->
     exists b', j b = Some (b', 0%Z) /\
           e2 ! i = Some (b', ty).
+
+Definition right_env_injection_none (e1 e2: env): Prop :=
+  forall i,
+    e1 ! i = None ->
+    e2 ! i = None.
+
+Definition right_env_injection (e1 e2: env): Prop :=
+  right_env_injection_some e1 e2 /\ right_env_injection_none e1 e2.
 
 Definition right_tenv_injection (le1 le2: temp_env): Prop :=
   forall i v,
@@ -71,10 +89,10 @@ Definition right_tenv_injection (le1 le2: temp_env): Prop :=
   [right_state_injection] should relate the context part of the two states, and ignore
   the program part of the two states.
   *)
-Variant right_executing_injection: state -> state -> Prop :=
+Variant right_executing_injection (ge1 ge2: genv): state -> state -> Prop :=
 | inject_states: forall f s k1 k2 e1 e2 le1 le2 m1 m2,
     (* we forget about program memories but require injection of context memories *)
-    right_mem_injection m1 m2 ->
+    right_mem_injection ge1 ge2 m1 m2 ->
 
     (* we forget about program parts of the continuation but require injection of
        context continuation *)
@@ -84,25 +102,25 @@ Variant right_executing_injection: state -> state -> Prop :=
     right_env_injection e1 e2 ->
     right_tenv_injection le1 le2 ->
 
-    right_executing_injection (State f s k1 e1 le1 m1) (State f s k2 e2 le2 m2)
+    right_executing_injection ge1 ge2 (State f s k1 e1 le1 m1) (State f s k2 e2 le2 m2)
 | inject_callstates: forall f vs k1 k2 m1 m2,
     (* we forget about program memories but require injection of context memories *)
-    right_mem_injection m1 m2 ->
+    right_mem_injection ge1 ge2 m1 m2 ->
 
     (* we forget about program parts of the continuation but require injection of
        context continuation *)
     right_cont_injection k1 k2 ->
 
-    right_executing_injection (Callstate f vs k1 m1) (Callstate f vs k2 m2)
+    right_executing_injection ge1 ge2 (Callstate f vs k1 m1) (Callstate f vs k2 m2)
 | inject_returnstates: forall v k1 k2 m1 m2 ty cp,
     (* we forget about program memories but require injection of context memories *)
-    right_mem_injection m1 m2 ->
+    right_mem_injection ge1 ge2 m1 m2 ->
 
     (* we forget about program parts of the continuation but require injection of
        context continuation *)
     right_cont_injection k1 k2 ->
 
-    right_executing_injection (Returnstate v k1 m1 ty cp) (Returnstate v k2 m2 ty cp)
+    right_executing_injection ge1 ge2 (Returnstate v k1 m1 ty cp) (Returnstate v k2 m2 ty cp)
 .
 
 Axiom is_left: split -> state -> Prop.
@@ -111,26 +129,26 @@ Axiom is_right: split -> state -> Prop.
 Axiom memory_of: state -> mem.
 Axiom cont_of: state -> cont.
 
-Variant right_state_injection: state -> state -> Prop :=
+Variant right_state_injection (ge1 ge2: genv): state -> state -> Prop :=
 | LeftControl: forall st1 st2,
     (* program (left) has control *)
     is_left s st1 ->
     is_left s st2 ->
 
     (* we forget about program memories but require injection of context memories *)
-    right_mem_injection (memory_of st1) (memory_of st2) ->
+    right_mem_injection ge1 ge2 (memory_of st1) (memory_of st2) ->
 
     (* we forget about program parts of the continuation but require injection of
        context continuation *)
     right_cont_injection (cont_of st1) (cont_of st2) ->
 
-    right_state_injection st1 st2
+    right_state_injection ge1 ge2 st1 st2
 | RightControl: forall st1 st2,
     (* context (right) has control *)
     is_right s st1 ->
     is_right s st2 ->
-    right_executing_injection st1 st2 ->
-    right_state_injection st1 st2.
+    right_executing_injection ge1 ge2 st1 st2 ->
+    right_state_injection ge1 ge2 st1 st2.
 
 
 End Equivalence.
@@ -138,13 +156,15 @@ End Equivalence.
 Section Simulation.
   Context (c p1 p2: Clight.program).
   Variable s: split.
-  Variable j: meminj.
+
 
   Context (ge1 ge2: genv).
+  (* Is this hypothesis realistic? *)
+  Hypothesis same_cenv: genv_cenv ge1 = genv_cenv ge2.
 
   Lemma eval_expr_lvalue_injection:
     forall s j m1 m2 e1 e2 le1 le2 cp,
-    forall inj: right_mem_injection s j m1 m2,
+    forall inj: right_mem_injection s j ge1 ge2 m1 m2,
     forall env_inj: right_env_injection j e1 e2,
     forall lenv_inj: right_tenv_injection j le1 le2,
     (forall a v,
@@ -159,7 +179,7 @@ Section Simulation.
                      eval_lvalue ge2 e2 cp le2 m2 a loc' (Ptrofs.add ofs (Ptrofs.repr ofs')) bf).
   Proof.
     intros.
-    destruct inj as [inj_dom inj_inject].
+    destruct inj as [inj_dom inj_inject j_delta_zero same_symb].
     apply eval_expr_lvalue_ind; intros;
     try now match goal with
     | |- exists _, Val.inject _ (Vint _) _ /\ _ => eexists; split; [eapply Val.inject_int | econstructor; eauto]
@@ -181,115 +201,145 @@ Section Simulation.
     - destruct H0 as [v1' [? ?]].
       destruct H2 as [v2' [? ?]].
       exploit sem_binary_operation_inject; eauto.
+      rewrite same_cenv.
       intros [? [? ?]].
       eexists; split; eauto.
       econstructor; eauto.
-    -
-    - (* this is a contradictory case: there is no unary operation that returns a pointer *)
-      destruct op; simpl in *.
-      + rewrite notbool_bool_val in H1.
-        destruct (bool_val _ _ _); [| congruence].
-        inv H1. now destruct b.
-      + unfold sem_notint in H1. destruct (classify_notint _); [| | congruence].
-        now destruct v1. now destruct v1.
-      + unfold sem_neg in H1. destruct (classify_neg _); try congruence; now destruct v1.
-      + unfold sem_absfloat in H1. destruct (classify_neg _); try congruence; now destruct v1.
-    - assert ((exists loc0 ofs0, v1 = Vptr loc0 ofs0) \/
-             (exists loc0 ofs0, v2 = Vptr loc0 ofs0)).
-      { destruct op; simpl in *.
-        - unfold sem_add in *.
-          destruct (classify_add _ _); simpl in *.
-          destruct v1, v2; simpl in *; destruct Archi.ptr64; simpl in *; inv H3; left; eexists; eexists; eauto.
-          destruct v1, v2; simpl in *; destruct Archi.ptr64; simpl in *; inv H3; left; eexists; eexists; eauto.
-          destruct v1, v2; simpl in *; destruct Archi.ptr64; simpl in *; inv H3; right; eexists; eexists; eauto.
-          destruct v1, v2; simpl in *; destruct Archi.ptr64; simpl in *; inv H3; right; eexists; eexists; eauto.
-          destruct (typeof a1), (typeof a2); unfold sem_binarith in *; simpl in *; try now inv H3.
-          destruct v1, v2; simpl in *.
-          unfold sem_binarith.
-
-
-            try (now
-              destruct v1, v2; simpl in *; destruct Archi.ptr64; simpl in *; inv H3; try (left; eexists; eexists; eauto);
-               try (right; eexists; eexists; eauto)).
-
-          destruct v2, v1; simpl in *; destruct Archi.ptr64; inv H3.
-            try now (eexists; eexists; eauto).
-
-            eexists; eexists; eauto.
-          + destruct v1, v2; simpl in *; destruct Archi.ptr64; simpl in *; inv H3.
-            eexists; eexists; eauto.
-            eexists; eexists; eauto.
-          +
-            simpl in H3.
-          destruct v1. simpl in H3.
-            try now destruct v1.
-          destruct v1; try now auto.
-
-        - rewrite notbool_bool_val in H1.
-          destruct (bool_val _ _ _); [| congruence].
-          inv H1. now destruct b.
-        - unfold sem_notint in H1. destruct (classify_notint _); [| | congruence].
-          now destruct v1. now destruct v1.
-        - unfold sem_neg in H1. destruct (classify_neg _); try congruence; now destruct v1.
-        - unfold sem_absfloat in H1. destruct (classify_neg _); try congruence; now destruct v1. }
-      subst v1.
-      specialize (H0 _ _ eq_refl) as [loc' [ofs' [? ?]]].
-      (* exploit sem_unary_operation_inject; eauto. *)
-      (* intros [tv [? ?]]. *)
-      (* destruct tv; try now inv H4. *)
-      (* inv H4. *)
-      exists loc', ofs'; split; eauto.
+    - destruct H0 as [v' [? ?]].
+      exploit sem_cast_inject; eauto.
+      intros [v1' [? ?]].
+      eexists; split; eauto.
       econstructor; eauto.
-      rewrite H3. congruence.
-    -
+    - rewrite same_cenv.
+      eexists; split; eauto.
+      econstructor; eauto.
+    - rewrite same_cenv.
+      eexists; split; eauto.
+      econstructor; eauto.
+    - destruct H0 as [loc' [ofs' [? ?]]].
+      (* This assert heavily relies on the assumption that the injection always gives a delta = 0. *)
+      assert (G: exists v', Val.inject j v v' /\
+                         deref_loc cp (typeof a) m2 loc' (Ptrofs.add ofs (Ptrofs.repr ofs')) bf v').
+      { inv H1.
+        - simpl in *.
+          exploit Mem.load_inject; eauto.
+          intros [v' [? ?]].
+          exploit j_delta_zero; eauto; intros; subst. rewrite Z.add_0_r in H1. rewrite Ptrofs.add_zero.
+          eexists; split; eauto. econstructor; simpl; eauto.
+        - exists (Vptr loc' (Ptrofs.add ofs (Ptrofs.repr ofs'))). split; eauto.
+          eapply deref_loc_reference; eauto.
+        - exists (Vptr loc' (Ptrofs.add ofs (Ptrofs.repr ofs'))). split; eauto.
+          eapply deref_loc_copy; eauto.
+        - inv H3.
+          exploit Mem.load_inject; eauto.
+          intros [v' [? ?]].
+          exploit j_delta_zero; eauto; intros; subst. rewrite Z.add_0_r in H3; rewrite Ptrofs.add_zero.
+          eexists; split; eauto.
+          eapply deref_loc_bitfield. inv H7.
+          econstructor; eauto. }
+      destruct G as [v' [? ?]].
+      eexists; split; eauto.
+      econstructor; eauto.
+    - destruct env_inj as [env_inj _].
+      exploit env_inj; eauto.
+      intros [b' [? ?]].
+      eexists; eexists; split; eauto.
+      econstructor; eauto.
+    - destruct env_inj as [_ env_inj].
+      exploit env_inj; eauto.
+      intros ?.
+      exploit same_symb; eauto.
+      intros [loc' [? ?]].
+      eexists; eexists; split; eauto.
+      eapply eval_Evar_global; eauto.
+    - destruct H0 as [v' [? ?]].
+      inv H0.
+      eexists; eexists; split; eauto.
+      econstructor; eauto.
+    - destruct H0 as [v' [? ?]].
+      inv H0.
+      eexists; eexists; split; eauto.
+      rewrite Ptrofs.add_assoc, (Ptrofs.add_commut (Ptrofs.repr delta)), <- Ptrofs.add_assoc.
+      eapply eval_Efield_struct; try rewrite <- same_cenv; eauto.
+    - destruct H0 as [v' [? ?]].
+      inv H0.
+      eexists; eexists; split; eauto.
+      rewrite Ptrofs.add_assoc, (Ptrofs.add_commut (Ptrofs.repr delta)), <- Ptrofs.add_assoc.
+      eapply eval_Efield_union; try rewrite <- same_cenv; eauto.
+  Qed.
 
+  Lemma eval_expr_injection:
+    forall s j m1 m2 e1 e2 le1 le2 cp,
+    forall inj: right_mem_injection s j ge1 ge2 m1 m2,
+    forall env_inj: right_env_injection j e1 e2,
+    forall lenv_inj: right_tenv_injection j le1 le2,
+    forall a v,
+      eval_expr ge1 e1 cp le1 m1 a v ->
+      exists v', Val.inject j v v' /\
+                     eval_expr ge2 e2 cp le2 m2 a v'.
+    Proof.
+      intros.
+      exploit eval_expr_lvalue_injection; eauto.
+      intros [? _]. eauto.
+    Qed.
 
-  Lemma parallel_concrete: forall s1 s2 s1' t,
-      right_state_injection s j s1 s2 ->
+  Lemma eval_lvalue_injection:
+    forall s j m1 m2 e1 e2 le1 le2 cp,
+    forall inj: right_mem_injection s j ge1 ge2 m1 m2,
+    forall env_inj: right_env_injection j e1 e2,
+    forall lenv_inj: right_tenv_injection j le1 le2,
+    forall a loc ofs bf,
+      eval_lvalue ge1 e1 cp le1 m1 a loc ofs bf ->
+      exists loc' ofs', j loc = Some (loc', ofs') /\
+                     eval_lvalue ge2 e2 cp le2 m2 a loc' (Ptrofs.add ofs (Ptrofs.repr ofs')) bf.
+    Proof.
+      intros.
+      exploit eval_expr_lvalue_injection; eauto.
+      intros [_ ?]. eauto.
+    Qed.
+
+  Lemma parallel_concrete: forall j s1 s2 s1' t,
+      right_state_injection s j ge1 ge2 s1 s2 ->
       is_right s s1 ->
       Clight.step1 ge1 s1 t s1' ->
-      exists s2',
+      exists j' s2',
         Clight.step1 ge2 s2 t s2' /\
-          right_state_injection s j s1' s2'.
+          right_state_injection s j' ge1 ge2 s1' s2'.
     Proof.
-      intros s1 s2 s1' t rs_inj is_r step1.
-      inv rs_inj.
+      intros j s1 s2 s1' t rs_inj is_r step1.
+      destruct rs_inj as [? | st1 st2 is_r1 is_r2 right_exec_inj].
+      (* inv rs_inj. *)
       - admit. (* contradiction *)
-      - inv step1; inv H1.
-        + assert (lemma1:
-                   right_mem_injection s j m m2 ->
-                   right_env_injection j e e2 ->
-                   right_tenv_injection j le le2 ->
-                   eval_lvalue ge1 e (comp_of f) le m a1 loc ofs bf ->
-                   exists loc' ofs', j loc = Some (loc', ofs') /\
-                          eval_lvalue ge2 e2 (comp_of f) le2 m2 a1 loc' (Ptrofs.add ofs (Ptrofs.repr ofs')) bf).
-          { clear.
-            intros inj env_inj lenv_inj ev.
-            destruct inj as [inj_dom inj_inject].
-            inv ev.
-            - exploit env_inj; eauto. intros [loc' [? ?]].
-              exists loc', 0%Z. split; eauto.
-              constructor; eauto.
-            - admit.
-            - eexists; eexists; split; eauto. admit.
-              constructor. admit.
-
-              admit.
-            - admit.
-            - admit.
-          }
-          exploit lemma1; eauto.
-          intros [loc' [ofs' [? ?]]].
-
-          eexists; split.
-          econstructor. eauto.
-          intros [loc' [ofs' [? ?]]].
-          eassumption.
-
-
-          admit. admit. admit. admit.
-          right. admit. admit.
-          econstructor; eauto. admit.
+      - inv step1; inv right_exec_inj.
+        Ltac destruct_mem_inj :=
+          match goal with
+          | H: right_mem_injection _ _ _ _ _ _ |- _ => destruct H as [same_dom mem_inject delta_zero same_symb]
+          end.
+        + exploit eval_lvalue_injection; eauto.
+          exploit eval_expr_injection; eauto.
+          intros [v' [? ?]] [loc' [ofs' [? ?]]].
+          destruct_mem_inj.
+          exploit sem_cast_inject; eauto.
+          intros [tv [? ?]].
+          inv H2.
+          * exploit Mem.store_mapped_inject; eauto.
+            intros [? [? ?]].
+            exploit delta_zero; eauto. intros ?; subst.
+            rewrite Z.add_0_r in *.
+            exists j; eexists; split.
+            -- econstructor; eauto.
+               econstructor; eauto.
+               rewrite Ptrofs.add_zero; eauto.
+            -- apply RightControl.
+               admit. admit.
+               constructor; eauto.
+               split; eauto.
+               clear -same_dom H10.
+               unfold same_domain in *.
+               intros. eapply same_dom.
+               erewrite <- Mem.store_block_compartment; eauto.
+          * admit.
+          * admit.
 Admitted.
 
 
